\begin{equation}
 F'(\theta) \appro	heta\frac{F(\theta+h)-F(\theta-h)}{2h} = 0 = F(\theta+h)-F(\theta-h)
\end{equation}

$F(\theta+h) = \frac{15}{0.6\sin{\theta+h}+\cos{\theta+h}} = \frac{15}{0.6\sin{\theta}\cos{h}+0.6\cos{\theta}\sin{h}+\cos{\theta}\cos{h}-\sin{\theta}\sin{h}} $
con $h = \frac{\pi}{2}$ 

$\Rightarrow F(\theta+h) = \frac{15}{0.6\cos{\theta}-\sin{\theta}}$

Por otro lado, al desarrollar el término anterior con $h = \frac{\pi}{2}$  tenemos

$F(\theta-h) = \frac{15}{0.6\sin{\theta-h}+\cos{\theta-h}} =  \frac{15}{-0.6\cos{\theta}+\sin{\theta}}$

Al sustituir en la fórmula (5)

$F(\theta+h)-F(\theta-h) = \frac{15}{0.6\cos{\theta}-\sin{\theta}} - \frac{15}{-0.6\cos{\theta}+\sin{\theta}} = \frac{-9\cos{\theta}+15\sin{\theta}-9\cos{\theta}+15\sin{\theta}}
{(0.6\cos{\theta}-\sin{\theta})(-0.6\cos{\theta}+\sin{\theta})} $

$\Rightarrow \frac{-18\cos{\theta}+30\sin{\theta}}
{(0.6\cos{\theta}-\sin{\theta})(-0.6\cos{\theta}+\sin{\theta})} = 0$ 

$\Rightarrow -18\cos{\theta}+30\sin{\theta} = 0$ $\Rightarrow 18\cos{\theta} = 30\sin{\theta} $ $\Rightarrow \frac{18}{30} = \tan{\theta} $ $\Rightarrow \Artan{18}{30} = \Artan{\theta} $ $\Rightarrow  \theta= 0.54041 $